context with var names and type judgement function

formalization/clerical/Typing.v
@@ -2,52 +2,12 @@
 
 Require Import Clerical.
 
-(* A typing context. *)
-Structure ctx := {
-  ctx_rw : list datatype ;
-  ctx_ro : list (list datatype)
-}.
-
-Definition empty_ctx := {| ctx_rw := nil; ctx_ro := nil |}.
-
-Definition extend t Γ :=
-  {| ctx_rw := cons t (ctx_rw Γ) ;
-     ctx_ro := ctx_ro Γ
-  |}.
-
-Definition readonly Γ :=
-  {|
-    ctx_rw := nil ;
-    ctx_ro := cons (ctx_rw Γ) (ctx_ro Γ)
-  |}.
-
 Open Scope clerical_scope.
 
-Inductive is_writable : list datatype -> nat -> datatype -> Type :=
-  | is_writable_0 :
-      forall Γ τ,
-        is_writable (cons τ Γ) 0 τ
-
-  | is_writable_S :
-      forall Γ τ σ k,
-        is_writable Γ k τ ->
-        is_writable (cons σ Γ) (S k) τ
-.
-
-Inductive has_type : ctx -> comp -> result_type -> Type :=
-  | has_type_Var_0 :
-      forall Γ τ,
-        has_type (extend τ Γ) (VAR 0) (RData τ)
-
-  | has_type_Var_S :
-      forall Γ σ τ k,
-        has_type Γ (VAR k) (RData τ) ->
-        has_type (extend σ Γ) (VAR (S k)) (RData τ)
-
-  | has_type_Var_empty_rw :
-      forall Γ τ k,
-        has_type Γ (VAR k) (RData τ) ->
-        has_type (readonly Γ) (VAR k) (RData τ)
+Inductive has_type : context -> comp -> result_type -> Type :=
+  | has_type_Var :
+    forall Γ s τ,
+      in_context_t Γ s τ -> has_type Γ (VAR s) (RData τ)
 
   | has_type_True :
       forall Γ,
@@ -73,7 +33,7 @@ Inductive has_type : ctx -> comp -> result_type -> Type :=
 
   | has_type_while :
       forall Γ b c,
-        has_type Γ b RBoolean ->
+        has_type (readonly  Γ) b RBoolean ->
         has_type Γ c RCommand ->
         has_type Γ (WHILE b DO c END) RCommand
 
@@ -86,17 +46,159 @@ Inductive has_type : ctx -> comp -> result_type -> Type :=
         has_type Γ (MCASE b1 ==> c1 OR b2 ==> c2 END) ρ
 
   | has_type_newvar :
-      forall Γ ρ τ e c,
+      forall Γ s ρ τ e c,
+        (in_context Γ s -> False) ->
         has_type (readonly Γ) e (RData τ) ->
-        has_type (extend τ Γ) c ρ ->
-        has_type Γ (NEWVAR e IN c) ρ
+        has_type (add_rw Γ s τ) c ρ ->
+        has_type Γ (NEWVAR s := e IN c) ρ
 
   | has_type_assign :
-      forall Γ τ k e,
-        is_writable (ctx_rw Γ) k τ ->
+      forall Γ s τ e,
+        in_context_trw Γ s τ true ->
         has_type (readonly Γ) e (RData τ) ->
-        has_type Γ (SET k := e) RCommand
+        has_type Γ (SET s := e) RCommand
 .
 
-(** TODO: a function which takes Γ and c and optionally gives the judgment [has_type Γ c t]
-    for some datatype [t]. *)
+
+(* Type checker: given a context it judeges type. if the given computation is not well-typed, it
+   leads to None. *)
+Fixpoint judge_type (Γ : context) (c : comp) : option result_type :=
+  match c with
+  | Var s => match locate Γ s with
+             | None => None
+             | Some v => let (a,b,c) := v in Some (RData b)
+             end 
+  | Boolean b => Some RBoolean
+  | Integer z => Some RInteger
+  | BinOp op a b => let τ :=  binary_op_type op (rev_type (judge_type (readonly Γ) a))
+                                                    (rev_type (judge_type (readonly Γ) b)) in
+                    match τ with
+                    | Some τ => Some ( RData τ )
+                    | None => None
+                    end
+  | UniOp op a => let τ := (unary_op_type op (rev_type (judge_type (readonly Γ) a))) in
+                  match τ with
+                  | Some τ => Some ( RData τ )
+                  | None => None
+                  end
+  | Skip => Some RCommand
+  | Sequence c1 c2 => let τ := (judge_type Γ c1) in
+                      match τ with
+                      | Some τ => match τ with
+                                  | RCommand => judge_type Γ c2
+                                  | _ => None
+                                  end
+                      | _ => None
+                      end
+  | Case b1 c1 b2 c2 => let Γ' := readonly Γ in
+                        let τ₁ := judge_type Γ' b1 in
+                        let τ₂ := judge_type Γ' b2 in
+                        match τ₁  with
+                        | Some RBoolean =>
+                          match τ₂ with
+                            | Some RBoolean => let ρ₁ := judge_type Γ c1 in
+                                                          let ρ₂ := judge_type Γ c2 in
+                                                          match ρ₁, ρ₂ with
+                                                          | Some ρ₁', Some ρ₂' => if (same_result_type ρ₁' ρ₂') then ρ₁ else None
+                                                          | _, _ => None
+                                                          end
+                            | _ => None
+                          end
+                            
+                        | _ => None
+                        end
+  | While b c => let τ := judge_type (readonly Γ) b in
+                 match τ with
+                 | Some RBoolean => let  ρ := judge_type Γ c in
+                                    match ρ with
+                                    | Some Rcommand => Some Rcommand
+                                    | _ => None
+                                    end
+                 | _ => None
+                 end
+                   
+  | Newvar s e c => if (is_in_context Γ s)
+                    then None
+                    else
+                      let τ := judge_type (readonly Γ) e in
+                      match τ with
+                      | Some τ => match τ with
+                                  | RData τ => judge_type (add_rw Γ s τ) c
+                                  | _ => None
+                                  end
+                      | _ => None
+                      end
+  | Assign s e => let v := locate Γ s in
+                  match v with
+                  | Some v => let (a,b,c) := v in
+                              if c then (
+                                  let ρ := judge_type (readonly Γ) e in
+                                  match ρ with
+                                  | Some ρ => if (same_result_type ρ (RData b)) then Some RCommand else None
+                                  | _ => None
+                                  end)
+                              else None
+                  | _ => None
+                  end
+  end.
+
+(* prove that the type judgement function is correct upto the inductive definition has_type *)
+Theorem Type_judgement_is_correct : forall Γ c τ, has_type Γ c τ -> judge_type Γ c = Some τ.
+Proof.
+Admitted.
+
+
+            
+
+
+
+
+
+
+
+            
+(* examples for type judgement *)
+Section type_examples.
+        
+  Definition Example1 :=
+    (
+      NEWVAR "x1" := INT 0 IN (* the accumulator is VAR 1 *)
+                         NEWVAR "x2" := VAR "x1" IN (* the counter is VAR 0 *)
+                                            WHILE (VAR "x1" <z INT 101) DO
+                                            (SET "x1" := (VAR "x2" +z VAR "x2") ;;
+                                                                                 SET "x2" := VAR "x1" +z INT 1)
+                                            END ;;
+                                            VAR "x2"
+    ).
+
+
+    Definition Example2 :=
+    (
+      NEWVAR "x1" := INT 0 IN (* the accumulator is VAR 1 *)
+                         NEWVAR "x2" := VAR "x1" IN (* the counter is VAR 0 *)
+                                            WHILE (VAR "x1" <z INT 101) DO
+                                            (SET "x1" := (VAR "x2" +z VAR "x2") ;;
+                                                                                 SET "x2" := VAR "x1" +z INT 1)
+                                            END
+    ).
+
+
+    (* Ill typed *)
+    Definition Example3 :=
+    (
+      (NEWVAR "x1" := INT 0 IN (* the accumulator is VAR 1 *)
+                         NEWVAR "x2" := VAR "x1" IN (* the counter is VAR 0 *)
+                                            WHILE (VAR "x1" <z INT 101) DO
+                                            (SET "x1" := (VAR "x2" +z VAR "x2") ;;
+                                                                                 SET "x2" := VAR "x1" +z INT 1)
+                                            END +z INT 5)
+    ).
+
+
+  
+
+  Eval compute in judge_type empty_context Example3.
+
+End type_examples.
+
+
